adds existential types and partial recusive type support

theories/lang/hazel.v
@@ -37,6 +37,50 @@ Notation "'list-match:' e1 'with' 'CONS' x => xs => e3 | 'NIL' => e2 'end'" :=
   (e1, x, xs, e2, e1 at level 200,
    format "'[hv' 'list-match:'  e1  'with'  '/  ' '[' 'CONS'  x  =>  xs  =>  '/  ' e3 ']'  '/' '[' |  'NIL'  =>  '/  ' e2 ']'  '/' 'end' ']'") : expr_scope.
 
+(* Notations for type abstraction and application *) 
+Notation "Λ: e" := (λ: <>, e)%E (at level 200, only parsing) : expr_scope.
+Notation "Λ: e" := (λ: <>, e)%V (at level 200, only parsing) : val_scope.
+Notation "e '<_>'" := (App e%E #()) (at level 10, only parsing) : expr_scope.
+
+(* Existential type packing and unpacking functions *)
+(* Since hazel is an untyped language there is no notion of packing a type 
+ * into an existential type nor unpacking an existential type.
+ * Instead we define pack/unpack as just the identity and application respectively
+ * to simply get a syntactic distinction for when existential pack/unpacking is applied *)
+Definition exist_pack : val := (λ: "x", "x")%V.
+Definition exist_unpack : val := (λ: "x" "y", "x" "y")%V.
+
+(* Notation for pack and unpack *)
+Notation "'pack:' e" := (exist_pack e%E)
+  (at level 200, e at level 200,
+   format "'[' 'pack:'  e ']'") : expr_scope.
+
+Notation "'unpack:' x := e1 'in' e2" := (exist_unpack (Lam x%binder e2%E) e1%E)
+  (at level 200, x at level 1, e1, e2 at level 200,
+   format "'[' 'unpack:'  x  :=  '[' e1 ']'  'in'  '/' e2 ']'") : expr_scope.
+Notation "'unpack:' x := e1 'in' e2" := (exist_unpack (LamV x%binder e2%E) e1%E)
+  (at level 200, x at level 1, e1, e2 at level 200,
+   format "'[' 'unpack:'  x  :=  '[' e1 ']'  'in'  '/' e2 ']'") : val_scope.
+
+(* Folding and unfolding recursive types *)
+(* Similarly as hazel is untyped we introduce the fold/unfold functions
+ * as being the identity functions.
+ * This gives us a syntactic distinction for when fold/unfold can be applied
+ * which is necessary to trigger a step in the operational semantics and thus
+ * remove the ▷ later modality in the recursive type definition. *)
+Definition rec_fold : val := (λ: "x", "x")%V.
+Definition rec_unfold : val := (λ: "x", "x")%V.
+
+(* Notations for fold and unfold *)
+Notation "'fold:' e" := (rec_fold e%E)
+  (at level 200, e at level 200,
+   format "'[' 'fold:'  e ']'") : expr_scope.
+
+Notation "'unfold:' e" := (rec_unfold e%E)
+  (at level 200, e at level 200,
+   format "'[' 'unfold:'  e ']'") : expr_scope.
+
+
 Global Instance load_atomic (l : loc) :
   Atomic StronglyAtomic (Load $ Val $ LitV $ LitLoc l).
 Proof.
